\subsection{Wick's theorem}

Use Wick's theorem to evaluate the following integrals.

\begin{enumerate}[(a)]
  \item $\int (x + y + z)^2 e^{-10x^2 - y^2 - 6xy - 2z^2} \dx\,\dy\,\dz$
\end{enumerate}

We have that:
\begin{align}
  c
   & =
  \int_{\R_n} \exp\left(-\frac{1}{2} \transpose{\vec{x}} \matr{A} \vec{x}\right) \dx^n =
  \left(\frac{(2\pi)^n}{\det\matr{A}}\right)^{1/2}
  \\[2ex]
  \avg{\cdots}
   & =
  \frac{1}{c} \int_{\R_n} \exp\left(-\frac{1}{2} \transpose{\vec{x}} \matr{A} \vec{x}\right) \cdots\,\dx^n
  \\[2ex]
  \avg{x_k x_\kp}
   & =
  (A^{-1})_{k \kp}
\end{align}

The exponent is:
\begin{align*}
  -10x^2 - y^2 - 6xy - 2z^2
   & =
  -\frac{1}{2}(20x^2 + 2y^2 + 12xy + 4z^2)
  \\
   & =
  -\frac{1}{2}
  \begin{bmatrix}
    x & y & z
  \end{bmatrix}
  \begin{bmatrix}
    20 & 6 & 0
    \\
    6  & 2 & 0
    \\
    0  & 0 & 4
  \end{bmatrix}
  \begin{bmatrix}
    x
    \\
    y
    \\
    z
  \end{bmatrix}
  \\
   & =
  -\frac{1}{2} \transpose{\vec{x}} \matr{A} \vec{x}
  \quad\text{where}\quad
  \vec{x} =
  \begin{bmatrix}
    x
    \\
    y
    \\
    z
  \end{bmatrix}
  ,\quad
  \matr{A} =
  \begin{bmatrix}
    20 & 6 & 0
    \\
    6  & 2 & 0
    \\
    0  & 0 & 4
  \end{bmatrix}
\end{align*}

Hence, with $\vec{x}$ and $\matr{A}$ as above, the integral is:
\begin{align}
   & \int_{\R^3} (x + y + z)^2 e^{-10x^2 - y^2 - 6xy - 2z^2} \dx\,\dy\,\dz
  \nonumber
  \\
   & \qquad =
  c \avg{(x + y + z)^2}
  \nonumber
  \\
   & \qquad =
  c \avg{x^2 + y^2 + z^2 + 2xy + 2xz + 2yz}
  \nonumber
  \\
   & \qquad =
  c \left(\avg{x^2} + \avg{y^2} + \avg{z^2} + 2\avg{xy} + 2\avg{xz} + 2\avg{yz}\right)
  \nonumber
  \\
   & \qquad =
  c \left((A^{-1})_{11} + (A^{-1})_{22} + (A^{-1})_{33} + 2(A^{-1})_{12} + 2(A^{-1})_{13} + 2(A^{-1})_{23}\right)
\end{align}

We also have that:
\begin{equation}
  \matr{A}^{-1} = \frac{1}{\det\matr{A}}\adj\matr{A}
\end{equation}
\begin{align*}
  \det\matr{A}
    & =
  20 (2 \times 4 - 0 \times 0) - 6 (6 \times 4 - 0 \times 0) + 0 (6 \times 0 - 2 \times 0)
  \\[2ex]
    & = 160 - 144 + 0 = 16
  \\[2ex]
  \adj\matr{A}
    & =
  \begin{bmatrix}
    2 \times 4 - 0 \times 0    & -(6 \times 4 - 0 \times 0)  & 6 \times 0 - 2 \times 0
    \\
    -(6 \times 4 - 0 \times 0) & 20 \times 4 - 0 \times 0    & -(20 \times 0 - 6 \times 0)
    \\
    6 \times 0 - 2 \times 0    & -(20 \times 0 - 6 \times 0) & 20 \times 2 - 6 \times 6
  \end{bmatrix}
  \\[2ex]
    & =
  \begin{bmatrix}
    8   & -24 & 0
    \\
    -24 & 80  & 0
    \\
    0   & 0   & 4
  \end{bmatrix}
  \\[2ex]
  \matr{A}^{-1}
    & = \frac{1}{16}
  \begin{bmatrix}
    8   & -24 & 0
    \\
    -24 & 80  & 0
    \\
    0   & 0   & 4
  \end{bmatrix}
  = \frac{1}{4}
  \begin{bmatrix}
    2  & -6 & 0
    \\
    -6 & 20 & 0
    \\
    0  & 0  & 1
  \end{bmatrix}
  \\[2ex]
  c & =
  \left(\frac{(2\pi)^3}{16}\right)^{1/2} = \sqrt{\frac{\pi^3}{2}}
\end{align*}
Finally, the integral is:
\begin{align*}
   & \int_{\R^3} (x + y + z)^2 e^{-10x^2 - y^2 - 6xy - 2z^2} \dx\,\dy\,\dz
  \\[2ex]
   & \qquad = \frac{c}{4}\left(2 + 20 + 1 + 2(-6) + 2(0) + 2(0)\right)
  = \frac{11}{4} \sqrt{\frac{\pi^3}{2}}
\end{align*}
