\newcommand{\xcl}{x_{\text{cl}}}
\newcommand{\xd}{\delta{x}}
\newcommand{\dxd}[1]{\text{d}\xd_{#1}}

\subsection{Propagator for a free particle}

Evaluate the path integral for the propagator of a particle moving freely in
one dimension without potential, i.e., a particle with the Lagrangian $L =
  \half m \dot{x}^2$.

The action is:
\begin{equation}
  \label{2.3-action}
  \func{S}{x} = \int_{0}^{t} \half m \dot{x}(\tp)^2 \dtp
\end{equation}
Split $x(\tp)$ into the classical solution $\xcl(\tp)$ and deviation $\xd(\tp)$:
\begin{equation}
  \label{2.3-decomposition}
  x(\tp) = \xcl(\tp) + \xd(\tp),\
  x(0) = x_0,\
  x(t) = x_f,\
  \xd(0) = \xd(t) = 0
\end{equation}
Substitute equation~\ref{2.3-decomposition} into equation~\ref{2.3-action}.
The Taylor expansion is around a stationary point of the action, so the linear
term vanishes:
\begin{align}
  \label{2.3-taylor}
  \func{S}{x}
   & =
  \int_{0}^{t} \half m \dot{\xcl}(\tp)^2 \dtp +
  \int_{0}^{t} m \dot{\xcl}(\tp)\dot{\xd}(\tp) \dtp +
  \int_{0}^{t} \half m \dot{\xd}(\tp)^2 \dtp
  \nonumber
  \\[2ex]
   & =
  \int_{0}^{t} \half m \dot{\xcl}(\tp)^2 \dtp +
  \int_{0}^{t} \half m \dot{\xd}(\tp)^2 \dtp
  \nonumber
  \\[3ex]
   & =
  \func{S}{\xcl} + \func{S}{\xd}
\end{align}
Substitute equation~\ref{2.3-taylor} into the path integral for the propagator and
replace the functional integral over $x$ by a functional integral over $\xd$:
\begin{align}
  \propone
   & = \int \func{D}{x} e^{\frac{i}{\hbar} \func{S}{x}} \nonumber
  \\
   & = \int \func{D}{x} e^{\frac{i}{\hbar} (\func{S}{\xcl} + \func{S}{\xd})} \nonumber
  \\
  \label{2.3-propagator}
   & = e^{\frac{i}{\hbar} \func{S}{\xcl}} \int \func{D}{\xd} e^{\frac{i}{\hbar} \func{S}{\xd}}
\end{align}
First, evaluate the action for the deviation:
\begin{equation*}
  \func{S}{\xd} = \int_{0}^{t} \half m \dot{\xd}(\tp)^2 \dtp
\end{equation*}
Discretise the integral and define $\tau = \frac{t}{N}$,
$\xd_i = \xd(\tp_i) = \xd(i\tau)$:
\begin{equation*}
  \func{S}{\xd}
  =
  \lim_{N \to \infty} \sum_{i=0}^{N-1} \half m \left(\frac{\xd_{i+1} - \xd_i}{\tau}\right)^2 \tau
  =
  \lim_{N \to \infty} \frac{m}{2\tau} \sum_{i=0}^{N-1} (\xd_{i+1}-\xd_i)^2
\end{equation*}
The boundary conditions $\xd(0) = \xd(t) = 0$ imply $\xd_0 = \xd_N = 0$.
Rearrange the sum:
\begin{align*}
  \sum_{i=0}^{N-1} (\xd_{i+1}-\xd_i)^2
   & =
  \sum_{i=0}^{N-1} \xd_{i+1}^2 -
  2\sum_{i=0}^{N-1} \xd_{i+1}\xd_i +
  \sum_{i=0}^{N-1} \xd_{i}^2
  \\[2ex]
   & =
  \sum_{i=0}^{N-2} \xd_{i+1}^2 -
  2\sum_{i=1}^{N-2} \xd_{i+1}\xd_i +
  \sum_{i=0}^{N-2} \xd_{i}^2
  \\[2ex]
   & =
  2\sum_{i=1}^{N-1} \xd_{i}^2 -
  2\sum_{i=1}^{N-2} \xd_{i+1}\xd_i
\end{align*}
In terms of the vector
$\vec{\xd} = \left[\xd_1\ \xd_2\ \dots\ \xd_{N-1}\right]^\top$
and Kronecker delta $\delta_{ij}$:
\begin{align*}
  \sum_{i=0}^{N-1} (\xd_{i+1}-\xd_i)^2
   & =
  \sum_{i=1}^{N-1} \sum_{j=1}^{N-1}
  \left(2\delta_{ij} - (\delta_{i+1,j}+\delta_{i,j+1})\right)
  (\vec{\xd})_{i}(\vec{\xd})_{j}
\end{align*}
\begin{equation*}
  \func{S}{\xd}
  =
  \lim_{N\to\infty}\frac{mN}{2t}\vec{\xd}\cdot\matr{B}_{N-1}\vec{\xd}
  \,,\quad
  \matr{B}_{N-1} =
  \begin{bmatrix}
    2      & - 1    & 0      & \cdots & 0
    \\
    -1     & 2      & -1     & \cdots & 0
    \\
    0      & -1     & 2      & \cdots & 0
    \\
    \vdots & \vdots & \vdots & \ddots & -1
    \\
    0      & 0      & 0      & -1     & 2
  \end{bmatrix}
\end{equation*}
The functional integral in equation~\ref{2.3-propagator} becomes:
\begin{multline}
  \label{2.3-deviation-action}
  \int \func{D}{\xd} e^{\frac{i}{\hbar} \func{S}{\xd}}
  =
  \lim_{N \to \infty}
  \left(\frac{mN}{2\pi i\hbar t}\right)^{N/2}
  \int\dxd{1}\int\dxd{2}\cdots
  \\
  \cdots\int\dxd{N-1}
  \exp\left(i \frac{mN}{2\hbar t} \vec{\xd}\cdot\matr{B}_{N-1}\vec{\xd}\right)
\end{multline}
We have that:
\begin{equation}
  \label{2.3-integral}
  \int\dxd{1}\int\dxd{2}\cdots\int\dxd{\nu-1}
  \exp\left(i\vec{\xd}\cdot\matr{A}\vec{\xd}\right)
  =
  \left(\frac{(i\pi)^\nu}{\det\matr{A}}\right)^{1/2}
\end{equation}
With $\nu = N-1$, $\matr{A} = \frac{mN}{2\hbar t} \matr{B}_{N-1}$:
\begin{equation*}
  \int \func{D}{\xd} e^{\frac{i}{\hbar} \func{S}{\xd}}
  =
  \lim_{N \to \infty}
  \left(\frac{mN}{2\pi i\hbar t}\right)^{N/2}
  \left(\frac{(i\pi)^{N-1}}{\det\left(\frac{mN}{2\hbar t}\matr{B}_{N-1}\right)}\right)^{1/2}
\end{equation*}
For a scalar $k$ and $n\times n$ matrix $A$, $\det k\matr{A} = k^n
  \det\matr{A}$.
Hence:
\begin{align}
  \int \func{D}{\xd} e^{\frac{i}{\hbar} \func{S}{\xd}}
   & =
  \lim_{N \to \infty}
  \left(\frac{mN}{2\pi i\hbar t}\right)^{N/2}
  \left(\frac{(i\pi)^{N-1}}{\left(\frac{mN}{2\hbar t}\right)^{N-1}\det\matr{B}_{N-1}}\right)^{1/2}
  \nonumber
  \\[2ex]
   & =
  \lim_{N \to \infty}
  \left(\frac{mN}{2\pi i\hbar t}\right)^{N/2}
  \left(\frac{2\pi i\hbar t}{mN}\right)^{(N-1)/2}
  \nonumber
  \\[2ex]
  \label{2.3-action-deviation}
   & =
  \sqrt{\frac{m}{2\pi i\hbar t}}
\end{align}
Next, evaluate the action for the classical solution.
The classical solution $\xcl(\tp)$ is the solution of Lagrange's equation:
\begin{equation*}
  \del[L]{x} = \ddt\del[L]{\dot{x}}
  \implies
  \ddot{\xcl}(\tp) = 0,\
  \dot{\xcl}(\tp) = \frac{x_f - x_0}{t}
\end{equation*}
The action for the classical solution is:
\begin{equation}
  \label{2.3-action-classical}
  \func{S}{\xcl} = \int_{0}^{t} \half m \dot{\xcl}(\tp)^2 \dtp
  = \half m \frac{\left(x_f - x_0\right)^2}{t}
\end{equation}
Substitute equations~\ref{2.3-action-deviation} and~\ref{2.3-action-classical}
into equation~\ref{2.3-propagator}:
\begin{equation}
  \label{2.3-result}
  \propone = \sqrt{\frac{m}{2\pi i\hbar t}}\exp\left(\ihbar\frac{m}{2t}(x_f - x_0)^2\right)
\end{equation}
